theories/Util/SemiDec.v
@@ -1,0 +1,127 @@
+Require Import ExtLib.Core.RelDec.
+Require Import ExtLib.Tactics.
+Require Import MirrorCore.Util.Compat.
+Require Import MirrorCore.Views.Ptrns.
+Require Import MirrorCore.Lambda.ExprCore.
+Require Import MirrorCore.Lambda.ExprD.
+Require Import MirrorCore.Lambda.RedAll.
+Require Import MirrorCore.Lambda.RewriteRelations.
+Require Import MirrorCore.Lambda.RewriteStrat.
+Require Import MirrorCore.Lambda.Red.
+Require Import MirrorCore.Lambda.Ptrns.
+Require Import MirrorCore.Lambda.Rewrite.HintDbs.
+Require Import MirrorCore.Reify.Reify.
+Require Import MirrorCore.RTac.IdtacK.
+Require Import MirrorCore.MTypes.ModularTypes.
+Require Import McExamples.PolyRewrite.MSimple.
+Require Import McExamples.PolyRewrite.MSimpleReify.
+
+(* TODO - many of the above imports are unnecessary *)
+
+(** Interface for semi-deciders (that use the RelDec typeclass)
+**)
+Section SemiDec.
+
+  Variable T : Type.
+  Variable equ : T -> T -> Prop.
+  Variable SD : RelDec equ.
+
+  Class RelDecSemiOk (SD : RelDec equ) : Prop :=
+    {
+      semi_dec_ok : forall (x y : T), rel_dec x y = true -> equ x y
+    }.
+
+  Section RelDec.
+
+    Variable RD : RelDec equ.
+    Variable RDC : RelDec_Correct RD.
+
+    
+    Print RelDec_Correct.
+    Check @rel_dec_correct.
+
+    Instance RelDecSemiOk_RelDec : RelDecSemiOk RD :=
+      { semi_dec_ok :=
+          fun x y => proj1 (@rel_dec_correct T equ RD RDC x y) }.
+  End RelDec.
+End SemiDec.  
+
+Section SemiDec_RSym.
+
+  (* need to have a typ *)
+  Variable typ : Type.
+  Variable typ_Rt : RType typ.
+  Variable func : Type.
+  Variable Rs : @RSym typ typ_Rt func.
+  Variable RsOk : RSymOk Rs.
+
+  Instance RelDecSemi_RSym : @RelDec func eq :=
+    { rel_dec x y :=
+        match @sym_eqb _ _ _ Rs x y with
+        | Some b => b
+        | _ => false
+        end
+    }.
+
+  Check RelDecSemiOk.
+  
+  Instance RelDecSemiOk_Rsym : RelDecSemiOk func _ RelDecSemi_RSym.
+  Proof.
+    destruct RsOk.
+    constructor. intros.
+    specialize (sym_eqbOk x y).
+    unfold rel_dec in H. simpl in H.
+    destruct (sym_eqb x y); subst; auto; congruence.
+  Qed.
+End SemiDec_RSym.
+
+Section SemiDec_expr.
+
+  Variable typ : Type.
+  Variable typ_Rt : RType typ.
+  Variable typ_RtOk : @RTypeOk typ typ_Rt.
+  Variable func : Type.
+  Variable func_Rs : @RSym typ typ_Rt func.
+  Variable func_RsOk : RSymOk func_Rs.
+
+  (* put SemiDec typeclass in util for now.
+     in the longer run,
+     Lambda/ExprCore.v should change to use SemiDec *)
+  Instance RelDecSemi_expr : RelDec (@eq (expr typ func)) :=
+    { rel_dec :=
+        expr_eq_dec (@ExprFacts.RelDec_eq_typ typ typ_Rt) (@RelDecSemi_RSym typ typ_Rt func func_Rs)
+    }.
+
+  Lemma expr_semi_dec_eq :
+    forall x y, expr_eq_dec ExprFacts.RelDec_eq_typ (RelDecSemi_RSym typ _ func func_Rs) x y = true ->
+           x = y.
+  Proof.
+    induction x; destruct y; try solve [intros; simpl in *; congruence].
+    { intros. simpl in *. 
+      apply EqNat.beq_nat_true in H. subst. reflexivity. }
+    { intros. simpl in *.
+      unfold rel_dec in H. simpl in H.
+      eapply sym_eqbOk with (a := f) (b := f0) in func_RsOk.
+      destruct (sym_eqb f f0) eqn:Heqb.
+      { subst; subst; reflexivity. }
+      { congruence. } }
+    { admit. (* can't figure out app case -- Mario *) }
+    { admit. (* or this one. *) }
+    { intros. simpl in *. apply EqNat.beq_nat_true in H. subst. reflexivity. }
+  Admitted.
+
+  (* put SemiDec inside of theories/Util *)
+  (* Do this: make a copy of Lambda that only uses MTypes *)
+  Instance SemiDecOk_expr : RelDecSemiOk (expr typ func) _ RelDecSemi_expr.
+  Proof.
+    constructor. intros.
+    unfold rel_dec in H. simpl in H.
+    apply expr_semi_dec_eq in H; auto.
+  Qed.
+End SemiDec_expr .
+
+
+Lemma RelDec_semidec {T} (rT : T -> T -> Prop)
+      (RDT : RelDec rT) (RDOT : RelDec_Correct RDT)
+: forall a b : T, a ?[ rT ] b = true -> rT a b.
+Proof. intros. consider (a ?[ rT ] b); auto. Qed.
